hash msg: stronger post condition & cleanup treehash proof

proof/correctness/FinalTreeHashProof.ec
@@ -20,7 +20,111 @@ require import WArray32.
 
 lemma eq_symm ['a] (a b : 'a) : a = b => b = a by move => ->.
 
-lemma treehash_correct ( _sk_seed _pub_seed : W8.t Array32.t, _s _t:W32.t, _addr:W32.t Array8.t): 
+op node_addr_padding_val : W32.t = W32.zero.
+
+module WOTS_GenLeaf = {
+  proc gen_leaf (sk_seed pub_seed : seed, address : W32.t Array8.t, s i : int) : nbytes = {
+    var node : nbytes; 
+    var pk : wots_pk;
+    pk <@ WOTS.pkGen(sk_seed, pub_seed, address);
+    address <- set_type address 1;
+    address <- set_ltree_addr address (s + i);
+    node <@ LTree.ltree(pk, address, pub_seed);
+    return node; 
+  }
+}.
+
+lemma gen_leaf_equiv (_sk_seed _pub_seed : W8.t Array32.t, x y : W32.t, oa lta a2 : W32.t Array8.t) : 
+    n = XMSS_N /\
+    d = XMSS_D /\
+    h = XMSS_FULL_HEIGHT /\
+    h %/d = XMSS_TREE_HEIGHT /\
+    w = XMSS_WOTS_W /\
+    len = XMSS_WOTS_LEN /\
+    n = XMSS_N /\
+    prf_padding_val = XMSS_HASH_PADDING_PRF /\
+    prf_kg_padding_val = XMSS_HASH_PADDING_PRF_KEYGEN /\
+    padding_len = XMSS_PADDING_LEN /\
+    F_padding_val = XMSS_HASH_PADDING_F =>
+    equiv [
+      M(Syscall).__gen_leaf_wots_ ~ WOTS_GenLeaf.gen_leaf :
+      
+      oa.[3] = W32.zero /\
+      lta.[3] = W32.one /\
+      lta.[4] = x + y /\
+      
+
+      sub lta 0 3 = sub a2 0 3 /\
+      sub oa 0 5 = sub a2 0 5 /\
+
+      arg{1}.`2 = _sk_seed /\
+      arg{1}.`3 = _pub_seed /\ 
+      arg{1}.`4 = lta /\
+      arg{1}.`5 = oa /\
+ 
+      arg{2}.`1 = NBytes.insubd (to_list _sk_seed) /\
+      arg{2}.`2 = NBytes.insubd (to_list _pub_seed) /\
+      arg{2}.`3 = a2 /\
+      arg{2}.`4 = to_uint x /\
+      arg{2}.`5 = to_uint y
+      ==> 
+
+      to_list res{1}.`1 = val res{2} /\
+      sub res{1}.`2 0 5 = sub lta 0 5 /\
+      sub res{1}.`3 0 5 = sub oa 0 5 
+    ].
+proof.
+rewrite /XMSS_N /XMSS_D /XMSS_TREE_HEIGHT /XMSS_FULL_HEIGHT /XMSS_D /XMSS_WOTS_W /XMSS_WOTS_LEN /= .
+move => [#] n_val d_val h_val tree_height *.
+rewrite h_val d_val in tree_height. 
+proc => /=.
+inline {1} 6.
+inline {1} 11.
+wp.
+
+seq 17 0 : (
+        sk_seed{2} = (insubd (to_list sk_seed1{1}))%NBytes /\
+        pub_seed{2} = (insubd (to_list pub_seed1{1}))%NBytes /\
+        s{2} = to_uint x /\ 
+        i{2} = to_uint y /\
+        ltree_addr1{1}.[3] = W32.one /\
+        ltree_addr1{1}.[4] = x + y /\
+        sub ltree_addr1{1} 0 3 = sub address{2} 0 3 /\
+        sub ots_addr1{1} 0 5 = sub address{2} 0 5 /\
+        ots_addr1{1}  = oa /\
+        ltree_addr1{1} = lta
+); first by auto.
+
+seq 1 1 : (
+  #{/~sub ots_addr1{1} 0 5 = sub address{2} 0 5}
+   {/~ots_addr1{1} = oa}pre /\
+  sub ots_addr1{1} 0 3 = sub address{2} 0 3 /\
+  sub ots_addr1{1} 0 5 = sub oa 0 5 /\
+  pk{2} = EncodeWotsPk pk{1}
+).
+    + exists * sk_seed1{1}, pub_seed1{1}, ots_addr1{1}, address{2}; elim * => P3 P4 P5 P6.
+      call {1} (pkgen_correct P3 P4 P5 P6 ) => [/# |].
+      skip => /> &1 &2 H0 H1 resL resR H2 H3. 
+      split; first by apply (eq_from_nth witness); rewrite !size_sub // => j?; rewrite !nth_sub // ; smt(sub_k).
+      by rewrite H2 -enc_dec_wots_pk.
+
+seq 0 2 : (
+  #pre /\
+  sub ltree_addr1{1} 0 5 = sub address{2} 0 5 
+).
+    + auto => /> &1 &2 H0 H1 H2 H3 H4.
+      rewrite /set_ltree_addr /set_type.
+      do split; (apply (eq_from_nth witness); rewrite !size_sub // => j?; rewrite !nth_sub //=).
+         * rewrite !get_setE // !ifF 1..6:/#; smt(sub_k).  
+         * rewrite !get_setE // !ifF 1..6:/#; smt(sub_k). 
+         * rewrite !get_setE //; case (j = 4) => [-> | ?]; first by smt(@W32 pow2_32).
+           case (j = 3) => [/# | ?]; rewrite !ifF 1..3:/#; smt(sub_k).
+ 
+exists * pk{1}, ltree_addr1{1}, pub_seed1{1}, address{2}; elim * => P0 P1 P2 P3.
+call (ltree_correct P0 P2 P1 P3) => [/# |]; auto => />.
+qed.
+
+lemma treehash_correct ( _sk_seed _pub_seed : W8.t Array32.t, _s _t: W32.t, a1 a2 : W32.t Array8.t): 
     n = XMSS_N /\
     d = XMSS_D /\
     h = XMSS_FULL_HEIGHT /\
@@ -39,17 +143,20 @@ lemma treehash_correct ( _sk_seed _pub_seed : W8.t Array32.t, _s _t:W32.t, _addr
       arg{1}.`3 = _pub_seed /\
       arg{1}.`4 = _s /\
       arg{1}.`5 = _t /\
-      arg{1}.`6 = _addr /\
+      arg{1}.`6 = a1 /\
       
       arg{2}.`1 = NBytes.insubd (to_list _pub_seed) /\
       arg{2}.`2 = NBytes.insubd (to_list _sk_seed) /\
       arg{2}.`3 = to_uint _s /\
       arg{2}.`4 = to_uint _t /\
-      arg{2}.`5 = _addr /\
+      arg{2}.`5 = a2 /\
 
       0 <= to_uint _t <= XMSS_TREE_HEIGHT /\
       0 <= to_uint _s <= to_uint _t /\
-      _addr.[4] = W32.zero
+
+      sub a1 0 3 = sub a2 0 3 /\
+      a1.[4] = node_addr_padding_val
+
       ==>
       to_list res{1} = val res{2}
     ]. 
@@ -61,57 +168,61 @@ rewrite h_val d_val in tree_height.
 proc => /=.
 have E0 : 2 ^ h = 1048576 by rewrite h_val /#.
 seq 7 0 : #pre; first by auto. 
+ 
 seq 4 3 : (
   #pre /\
   offset{1} = W64.zero /\
   ={offset} /\
-  ots_addr{1} = subtree_addr{1} /\
-  ltree_addr{1} = subtree_addr{1} /\
-  node_addr{1} = subtree_addr{1} /\
-  node_addr{1}.[4] = W32.zero /\
-  address{2}.[4] = W32.zero /\
+  sub ots_addr{1}   0 3 = sub subtree_addr{1} 0 3 /\
+  sub ltree_addr{1} 0 3 = sub subtree_addr{1} 0 3 /\
+  sub node_addr{1}  0 3 = sub subtree_addr{1} 0 3 /\
+
+  sub ots_addr{1}   0 3 = sub a1 0 3 /\
+  sub ltree_addr{1} 0 3 = sub a1 0 3 /\
+  sub node_addr{1}  0 3 = sub a1 0 3 /\
+
+  node_addr{1}.[4] = node_addr_padding_val /\
 
   size stack{2} = h %/ d + 1 /\      (* = 11 *)
   size heights{2} = h %/ d + 1  /\   (* = 11 *)
   size stack{2} = size heights{2}
 ).
-    + auto => /> ???? H; do split; 5,6: by rewrite size_nseq /#.
-         * rewrite tP => j*.
-           rewrite initiE //= get32E pack4E wordP => i?.
+    + auto => /> *. 
+      do split; try (apply (eq_from_nth witness); rewrite !size_sub // => j?; rewrite !nth_sub //= initiE //= 1:/#).
+         * rewrite get32E pack4E wordP => i?.
            rewrite initiE //= initiE 1:/# /= /init64 initiE 1:/# /= /copy_64 initiE 1:/# /=.
-           rewrite  get64E pack8E bits8iE 1:/# initiE 1:/# /= initiE 1:/# //= /init32 initiE 1:/# /= bits8iE /#.
-         * rewrite tP => j*.
-           rewrite initiE //= get32E pack4E wordP => i?.
+           rewrite get64E pack8E bits8iE 1:/# initiE 1:/# /= initiE 1:/# //= /init32 initiE 1:/# /= bits8iE /#.
+         * rewrite get32E pack4E wordP => i?.
            rewrite initiE //= initiE 1:/# /= /init64 initiE 1:/# /= /copy_64 initiE 1:/# /=.
-           rewrite  get64E pack8E bits8iE 1:/# initiE 1:/# /= initiE 1:/# //= /init32 initiE 1:/# /= bits8iE /#.
-         * rewrite tP => j*.
-           rewrite initiE //= get32E pack4E wordP => i?.
+           rewrite get64E pack8E bits8iE 1:/# initiE 1:/# /= initiE 1:/# //= /init32 initiE 1:/# /= bits8iE /#.
+         * rewrite get32E pack4E wordP => i?.
            rewrite initiE //= initiE 1:/# /= /init64 initiE 1:/# /= /copy_64 initiE 1:/# /=.
-           rewrite  get64E pack8E bits8iE 1:/# initiE 1:/# /= initiE 1:/# //= /init32 initiE 1:/# /= bits8iE /#.
-         * rewrite /get32_direct pack4E wordP => i?.
+           rewrite get64E pack8E bits8iE 1:/# initiE 1:/# /= initiE 1:/# //= /init32 initiE 1:/# /= bits8iE /#.
+         * rewrite get32E pack4E wordP => i?.
            rewrite initiE //= initiE 1:/# /= /init64 initiE 1:/# /= /copy_64 initiE 1:/# /=.
-           rewrite  get64E pack8E bits8iE 1:/# initiE 1:/# /= initiE 1:/# //= /init32 initiE 1:/# /= bits8iE 1:/#.
-           rewrite (: (8 * ((16 + i %/ 8) %/ 8) + ((16 + i %/ 8) %% 8 * 8 + i %% 8) %/ 8) %/ 4 = 4) 1:/# H /#.
-         * by rewrite !size_nseq. 
+           rewrite get64E pack8E bits8iE 1:/# initiE 1:/# /= initiE 1:/# //= /init32 initiE 1:/# /= bits8iE /#.
+         * rewrite get32E pack4E wordP => i?.
+           rewrite initiE //= initiE 1:/# /= /init64 initiE 1:/# /= /copy_64 initiE 1:/# /=.
+           rewrite get64E pack8E bits8iE 1:/# initiE 1:/# /= initiE 1:/# //= /init32 initiE 1:/# /= bits8iE /#.
+         * rewrite get32E pack4E wordP => i?.
+           rewrite initiE //= initiE 1:/# /= /init64 initiE 1:/# /= /copy_64 initiE 1:/# /=.
+           rewrite get64E pack8E bits8iE 1:/# initiE 1:/# /= initiE 1:/# //= /init32 initiE 1:/# /= bits8iE /#.
+         * rewrite get32E pack4E wordP => i?.
+           rewrite initiE //= initiE 1:/# /= /init64 initiE 1:/# /= /copy_64 initiE 1:/# /=.
+           rewrite get64E pack8E bits8iE 1:/# initiE 1:/# /= initiE 1:/# //= /init32 initiE 1:/# /= bits8iE /#.
+         * by rewrite size_nseq h_val d_val /=.
+         * by rewrite size_nseq h_val d_val /=.
+         * by rewrite !size_nseq h_val d_val /=.
 
 seq 4 0 : (
-  #{/~ots_addr{1} = subtree_addr{1}}
-   {/~ltree_addr{1} = subtree_addr{1}}
-   {/~node_addr{1} = subtree_addr{1}}pre /\
-   sub ots_addr{1} 0 3 = sub address{2} 0 3 /\ 
-   sub ltree_addr{1} 0 3 = sub address{2} 0 3 /\
-   sub node_addr{1} 0 3 = sub address{2} 0 3 /\
+   #pre /\
    ots_addr{1}.[3] = W32.zero /\
    ltree_addr{1}.[3] = W32.one /\
-   node_addr{1}.[3] = W32.of_int 2 /\
-   node_addr{1}.[4] = W32.zero
+   node_addr{1}.[3] = W32.of_int 2 
 ).
     + inline {1}.
       auto => /> *.
-      do split; (
-          apply (eq_from_nth witness); [by rewrite !size_sub | rewrite size_sub // => ??]; 
-          by rewrite !nth_sub //= get_setE // ifF 1:/# 
-      ).
+      do split; (apply (eq_from_nth witness); rewrite !size_sub // => j?; rewrite !nth_sub // get_setE // ifF 1:/# /=; smt(sub_k)).
 
 swap {1} 1 2.
 
@@ -145,138 +256,58 @@ seq 2 2 : (sub _stack{1} 0 n = val (nth witness stack{2} 0)); last first.
 
 unroll {1} 2; unroll {2} 2.
 sp 1 1.
-rcondt {1} 1.
-      + auto => /> &hr ???????????????H.
-        rewrite ultE H /=. 
-        by apply pow2_pos.
-rcondt {2} 1.
-      + auto => &hr *.
-        smt(pow2_pos).
 
+rcondt {1} 1; first by auto => /> &hr ????????????????H; rewrite ultE H /=; apply pow2_pos.
+rcondt {2} 1; first by auto => &hr *; smt(pow2_pos).
+  
 seq 2 0 : (#pre /\ to_uint t32{1} = s{2} + i{2}); first by auto.
 
 swap {1} 2 -1.
 
-seq 1 2 : ( 
-    #{/~sub ots_addr{1} 0 3 = sub address{2} 0 3}
-     {/~address{2} = _addr}
-     {/~address{2}.[4] = W32.zero}pre /\ 
+seq 1 2 : (  
+     #{/~address{2} = a2}pre /\ 
      sub ots_addr{1} 0 5 = sub address{2} 0 5
-).
+). 
+    + inline {1}; auto => /> &1 &2 *.  
+      rewrite /set_type /set_ots_addr.
+      do split; (apply (eq_from_nth witness); rewrite !size_sub // => j?; rewrite !nth_sub // get_setE //).
+         * do (rewrite ifF 1:/#); smt(sub_k).
+         * smt(sub_k).
+         * case (j = 4) => [-> //= | ?]; first by smt(@W32 pow2_32).
+           rewrite ifF 1:/# /= get_setE // ifF 1:/#. 
+           rewrite !get_setE // ifF 1:/# ifF 1:/# ifF 1:/# ifF 1:/#.
+           smt(sub_k).
+
+seq 1 0 : (#pre /\ ltree_addr{1}.[4] = t32{1}).
+    + inline {1}; auto => /> &1 &2 *.
+      split; apply (eq_from_nth witness); rewrite !size_sub // => j?; rewrite !nth_sub //= get_setE // ifF 1:/#; smt(sub_k).
+
+outline {2} [1-4] { node <@ WOTS_GenLeaf.gen_leaf (sk_seed, pub_seed, address, s, i); }.
+
+seq 0 0 : (#pre /\ sub ltree_addr{1} 0 3 = sub address{2} 0 3).
+    + auto => /> *; apply (eq_from_nth witness); rewrite !size_sub // => j?; rewrite !nth_sub //; smt(sub_k).
  
-    + inline {1}; auto => /> &1 &2 H0 H1 H2 H3 H4 H5 H6 H7 H8 H9 H10 H11 H12 H13 H14 H15 H16.  
-      do split; (
-         apply (eq_from_nth witness); [by rewrite !size_sub | rewrite size_sub // => j?];
-         rewrite !nth_sub //= !get_setE //
-      ).
-         * do (rewrite ifF 1:/#).
-           have ->: ltree_addr{1}.[j] = nth witness (sub ltree_addr{1} 0 3) j by rewrite nth_sub.
-           by rewrite H10 nth_sub.
-         * do (rewrite ifF 1:/#).
-           have ->: node_addr{1}.[j] = nth witness (sub node_addr{1} 0 3) j by rewrite nth_sub.
-           by rewrite H11 nth_sub.
-         * case (j = 4) => ?.
-              - smt(@W32 pow2_32).
-              - do 3! (rewrite ifF 1:/#).
-                case (j = 3) => [/# |?].
-                have ->: ots_addr{1}.[j] = nth witness (sub ots_addr{1} 0 3) j by rewrite nth_sub /#.
-                rewrite H9 nth_sub /#.
-
-seq 1 0 : (#pre /\ ltree_addr{1}.[4] = W32.of_int (s{2} + i{2})).
-    + inline {1}; auto => /> &1 &2 H0 H1 H2 H3 H4 H5 H6 H7 H8 H9 H10 H11 H12 H13 H14 H15 H16. 
-      split.
-         * apply (eq_from_nth witness); first by rewrite !size_sub.
-           rewrite size_sub // => i?.
-           rewrite !nth_sub // get_setE // ifF 1:/# /=.
-           have ->: ltree_addr{1}.[i] = nth witness (sub ltree_addr{1} 0 3) i by rewrite nth_sub.
-           by rewrite H9 nth_sub.
-         * smt(@W32 pow2_32).
-
-seq 1 4 : (
-  #{/~sub ots_addr{1} 0 5 = sub address{2} 0 5}
-   {/~ltree_addr{1}.[4] = (of_int (s{2} + i{2}))%W32}pre /\
+seq 1 1 : (
+  #{/~sub ots_addr{1} 0 5 = sub address{2} 0 5} 
+   {/~ltree_addr{1}.[4] = (of_int s{2})%W32}pre /\
    val node{2} = to_list buf{1} /\ 
-   sub ots_addr{1} 0 3 = sub address{2} 0 3
+   sub ots_addr{1} 0 5 = sub address{2} 0 5
 ).
-
-(* ================================================== proof for gen leaf starts here =================================================================== *)
-
-inline {1} M(Syscall).__gen_leaf_wots_ M(Syscall)._gen_leaf_wots M(Syscall).__gen_leaf_wots.             
-
-seq 22 0 : (
-    #pre /\
-  sk_seed2{1} = sk_seed{1} /\
-  pub_seed2{1} = pub_seed{1} /\
-  ots_addr2{1} = ots_addr{1} /\
-  ltree_addr2{1} = ltree_addr{1}
-); first by auto.
-
-seq 1 1 : (
-        #{/~ots_addr2{1} = ots_addr{1}}pre /\ 
-        pk{1} = DecodeWotsPk pk{2} /\
-        ots_addr2{1}.[0] = address{2}.[0] /\
-        ots_addr2{1}.[1] = address{2}.[1] /\
-        ots_addr2{1}.[2] = address{2}.[2] /\
-        ots_addr2{1}.[3] = W32.zero 
-).
-         * exists * sk_seed2{1}, pub_seed2{1}, ots_addr2{1}, address{2}.
-           elim * => P3 P4 P5 P6.
-           call {1} (pkgen_correct P3 P4 P5 P6) => [/# |].
-           auto => /> &1 &2 H0 H1 H2 H3 H4 H5 H6 H7 H8 H9 H10 H11 H12 H13 H14 H15 H16 H17 resultL resultR H18 H19.
-           do split; [
-               have ->: P6.[0] = nth witness (sub P6 0 5) 0 by rewrite nth_sub | 
-               have ->: P6.[1] = nth witness (sub P6 0 5) 1 by rewrite nth_sub |     
-               have ->: P6.[2] = nth witness (sub P6 0 5) 2 by rewrite nth_sub |
-           ]; 1..3: by  rewrite -H17 -H19 nth_sub /#.        
-           have ->: resultL.`2.[3] = nth witness (sub resultL.`2 0 5) 3 by rewrite nth_sub /#.
-           by rewrite H19 nth_sub.
-
-seq 0 2 : (
-          #{/~sub ots_addr{1} 0 5 = sub address{2} 0 5}pre /\ 
-          sub ltree_addr2{1} 0 5 = sub address{2} 0 5
-      ).
-         * auto => /> &1 &2 H0 H1 H2 H3 H4 H5 H6 H7 H8 H9 H10 H11 H12 H13 H14 H15 H16 H17 H18 H19 H20. 
-           rewrite /set_ltree_addr /set_type.
-           do split; (
-              apply (eq_from_nth witness); [by rewrite !size_sub | rewrite size_sub // => i?];
-              rewrite !nth_sub // !get_setE //=
-           ).
-               - do (rewrite ifF 1:/#).
-                 have ->: ltree_addr{1}.[i] = nth witness (sub ltree_addr{1} 0 3) i by rewrite nth_sub.
-                 by rewrite H9 nth_sub.
-               - do (rewrite ifF 1:/#).
-                 have ->: node_addr{1}.[i] = nth witness (sub node_addr{1} 0 3) i by rewrite nth_sub.
-                 by rewrite H10 nth_sub.
-               - case (i = 4) => [-> /# |?].
-                 case (i = 3) => [-> /# |?].
-                 do (rewrite ifF 1:/#).
-                 have ->: ltree_addr{1}.[i] = nth witness (sub ltree_addr{1} 0 3) i by rewrite nth_sub /#.
-                 by rewrite H9 nth_sub /#.
-
-seq 1 1 : (
-          #{/~ltree_addr2{1} = ltree_addr{1}}pre /\ 
-          to_list leaf1{1} = val node{2} /\
-          ltree_addr2{1}.[0] = address{2}.[0] /\
-          ltree_addr2{1}.[1] = address{2}.[1] /\
-          ltree_addr2{1}.[2] = address{2}.[2] /\
-          ltree_addr2{1}.[3] = W32.one
-      ).
-         * exists * pk{1}, ltree_addr2{1}, pub_seed2{1}.
-           elim * => P0 P1 P2.
-           call (ltree_correct P0 P2 P1) => [/# |].
-           auto => /> &1 &2 *; split; [apply enc_dec_wots_pk => /# | smt(addr_sub_5)].
-
-auto => /> &1 &2 H0 H1 H2 H3 H4 H5 H6 H7 H8 H9 H10 H11 H12 H13 H14 H15 H16 H17 H18 H19 H20 H21 H22 H23 H24 H25.
-      do split.
-         * apply (eq_from_nth witness); first by rewrite !size_sub.
-           rewrite size_sub // => i?. 
-           rewrite !nth_sub /#.
-         * by rewrite H21.
-         * apply (eq_from_nth witness); first by rewrite !size_sub.
-           rewrite size_sub // => i?. 
-           rewrite !nth_sub /#.
-
-(* ================================================== proof for gen leaf ends here =================================================================== *)
+    + exists * sk_seed{1}, pub_seed{1}, (of_int s{2})%W32, (of_int i{2})%W32, ots_addr{1}, ltree_addr{1}, address{2}.
+      elim * => P0 P1 P2 P3 P4 P5 P6.
+      call (gen_leaf_equiv P0 P1 P2 P3 P4 P5 P6) => [/# |].
+      skip => /> &1 &2 *; split; first by smt(@W32 pow2_32).
+      move => *; do split.
+        - apply (eq_from_nth witness); rewrite !size_sub // => j?; rewrite !nth_sub //; smt(sub_k). 
+        - apply (eq_from_nth witness); rewrite !size_sub // => j?; rewrite !nth_sub //; smt(sub_k).         
+        - apply (eq_from_nth witness); rewrite !size_sub // => j?; rewrite !nth_sub //; smt(sub_k). 
+        - apply (eq_from_nth witness); rewrite !size_sub // => j?; rewrite !nth_sub //; smt(sub_k). 
+        - smt(sub_k).
+        - smt(sub_k).
+        - smt(sub_k).
+        - apply (eq_from_nth witness); rewrite !size_sub // => j?; rewrite !nth_sub //; smt(sub_k). 
+        - smt(@NBytes).
+        - smt(sub_k).
 
 seq 3 1 : (
     #pre /\ 
@@ -286,13 +317,12 @@ seq 3 1 : (
     + exists * buf{1}, stack{2}, _stack{1}, offset{1}.
       elim * => P0 P1 P2 P3. 
       sp.
-      call {1} (p_treehash_memcpy P0 P1 P2 P3) => [/# |].
-      skip => /> &1 &2 H0 H1 H2 H3 H4 H5 H6 H7 H8 H9 H10 H11 H12 H13 H14 H15 H16 H17. 
-      do split. 
+      call {1} (p_treehash_memcpy_0 P0 P1 P2 P3) => [/# |].
+      skip => /> &1 &2 H0 H1 H2 H3 H4 H5 H6 H7 H8 H9 H10 H11 H12 H13 H14 H15 H16 H17 H18 *. 
+      do split.
         - smt().
         - apply (eq_from_nth witness); first by rewrite size_sub 1:/# size_sub_list /#.
-          rewrite size_sub 1:/# /XMSS_N (: 32 * min 0 (size P1) = 0) 1:/# => j?.
-          smt().
+          by rewrite size_sub /#.
         - move => H24 H25 result H26.
           rewrite size_put; split => //. (* the first goal of split is solved by trivial *)
           apply (eq_from_nth witness); first by rewrite size_sub 1:/# size_sub_list /#.
@@ -302,8 +332,6 @@ seq 3 1 : (
           rewrite H26.
           do congr.
           smt(@NBytes).
- 
-conseq />.
 
 seq 1 1 : ( 
   #{/~sub _stack{1} 0 (n * (to_uint offset{2} + 1)) = sub_list (nbytes_flatten stack{2}) 0 (n * (to_uint offset{2} + 1))}
@@ -321,8 +349,7 @@ seq 1 1 : (#pre /\ sub heights{1} 0 1 = sub_list heights{2} 0 1).
       rewrite get_setE //= nth_put //=/#.
 
 seq 1 0 : (#pre /\ cond{1} = W8.zero).
-    + ecall {1} (p_treehash_condition_if heights{1} offset{1}).
-      auto => /> &1 &2 *.
+    + ecall {1} (p_treehash_condition_if heights{1} offset{1}); auto => />.
 
 rcondf {2} 2; first by auto.
 rcondf {1} 1; first by auto => /> *; smt(@W8).
@@ -334,13 +361,10 @@ seq 1 1 : (
     i{2} = 1
 ); first by auto.
 
-seq 0 1 : #pre.
+seq 0 1 : #{/~sub ots_addr{1} 0 5 = sub address{2} 0 5}pre.
     + auto => /> &1 &2 *.
-      do split; (
-      apply (eq_from_nth witness); [by rewrite !size_sub // | rewrite size_sub // => j?];
-      rewrite !nth_sub //= !get_setE //;
-      do rewrite ifF 1:/#; smt(sub_k)     
-    ).
+      rewrite /set_type.
+      apply (eq_from_nth witness); rewrite !size_sub // => j?; rewrite !nth_sub //= !get_setE // !ifF 1..5:/#; smt(sub_k).
 
 while (
       t{2} = to_uint target_height{1} /\ 0 <= t{2} <= h /\
@@ -365,26 +389,24 @@ while (
       ots_addr{1}.[3] = W32.zero /\       (* type *)
       ltree_addr{1}.[3] = W32.one /\      (* type *)
       node_addr{1}.[3] = W32.of_int 2 /\  (* type *)
-      node_addr{1}.[4] = W32.zero /\      (* padding *)
+      node_addr{1}.[4] = node_addr_padding_val /\
       
       sub heights{1} 0 (min (to_uint offset{2}) (size heights{2})) = sub_list heights{2} 0 (min (to_uint offset{2}) (size heights{2})) /\
 
       sub _stack{1} 0 (n * (min (to_uint offset{2}) (size stack{2}))) = sub_list (nbytes_flatten stack{2}) 0 (n * (min (to_uint offset{2}) (size stack{2})))
 ); last first.
-
-(* ============= LAST SUBGOAL OF (the first) WHILE STARTS HERE ============= *)
-
 + auto => /> &1 &2 H0 H1 H2 H3 H4 H5 H6 H7 H8 H9 H10 H11 H12 H13 H14 *.
   do split; 1,2: by smt().
-        * apply pow2_leq_1. 
-        * apply H0.
+        * by apply pow2_leq_1; apply H0. 
+        * apply (eq_from_nth witness); rewrite !size_sub // => j?; rewrite !nth_sub //; smt(sub_k). 
+        * apply (eq_from_nth witness); rewrite !size_sub // => j?; rewrite !nth_sub //; smt(sub_k). 
         * apply (eq_from_nth witness); first by rewrite size_sub 1:/# size_sub_list /#.
           rewrite size_sub /#.
         * apply (eq_from_nth witness); first by rewrite size_sub 1:/# size_sub_list /#.
           rewrite  size_sub /#.
-        - rewrite ultE /#.
-        - rewrite ultE /#.
-        - move => stackL heightsL iL ltree_addrL node_addrL ots_addrL addressR heightsR offsetR stackR.      
+        * rewrite ultE /#.
+        * rewrite ultE /#.
+        * move => stackL heightsL iL ltree_addrL node_addrL ots_addrL addressR heightsR offsetR stackR.      
           rewrite ultE => H15 H16 H17 H18 H19 H20 H21 H22 H23 H24 H25 H26 H27 H28 H29 H30 H31 H32 H33 *.
           apply (eq_from_nth witness); first by rewrite size_sub 1:/# valP n_val.
           rewrite size_sub 1:/# n_val => j?.
@@ -396,15 +418,13 @@ while (
           rewrite T nth_mkseq /=; first by smt(@W64 pow2_64).
           rewrite nth_nbytes_flatten /#.
 
-(* ============= LAST SUBGOAL OF (the first) WHILE ENDS HERE ============= *)
-
 (* ============= FIRST SUBGOAL OF WHILE STARTS HERE ============= *)
 
-seq 2 0 : (#pre /\ to_uint t32{1} = s{2} + i{2}).
-    + auto => /> &1 &2; rewrite ultE => *.
-      rewrite to_uintD_small //=. 
-      smt(@IntDiv @RealExp).
+outline {2} [3-6] { node <@ WOTS_GenLeaf.gen_leaf (sk_seed, pub_seed, address, s, i); }.
  
+seq 2 0 : (#pre /\ to_uint t32{1} = s{2} + i{2}).
+    + auto => /> &1 &2; rewrite ultE => *; rewrite to_uintD_small //=; smt(@IntDiv @RealExp).
+
 swap {1} 2 -1.
 
 seq 1 2 : (
@@ -429,106 +449,31 @@ seq 1 2 : (
                 have ->: ots_addr{1}.[j] = nth witness (sub ots_addr{1} 0 3) j by rewrite nth_sub /#.
                 rewrite H11 nth_sub /#.
 
-wp.
-
 seq 1 0 : (#pre /\ ltree_addr{1}.[4] = W32.of_int (s{2} + i{2})).
     + inline {1}; auto => /> &1 &2 H0 H1 H2 H3 H4 H5 H6 H7 H8 H9 H10 H11 H12 H13 H14 H15 H16 H17 H18 H19 H20 H21 *.
-      split.
-         * apply (eq_from_nth witness); first by rewrite !size_sub.
-           rewrite size_sub // => i?.
-           rewrite !nth_sub // get_setE // ifF 1:/# /=.
-           have ->: ltree_addr{1}.[i] = nth witness (sub ltree_addr{1} 0 3) i by rewrite nth_sub.
-           by rewrite H11 nth_sub.
-         * by rewrite -H21 to_uintK.
+      split; last by smt(@W32 pow2_32).
+      apply (eq_from_nth witness); rewrite !size_sub // => i?; rewrite !nth_sub // get_setE // ifF 1:/#; smt(sub_k).
 
-seq 1 4 : (
-  #{/~sub ots_addr{1} 0 5 = sub address{2} 0 5}
-   {/~ltree_addr{1}.[4] = (of_int (s{2} + i{2}))%W32}pre /\
+wp; conseq />.
+
+seq 1 1 : (
+  #{/~sub ots_addr{1} 0 5 = sub address{2} 0 5} 
+   {/~ltree_addr{1}.[4] = (of_int s{2})%W32}pre /\
    val node{2} = to_list buf{1} /\ 
-   sub ots_addr{1} 0 3 = sub address{2} 0 3
+   sub ots_addr{1} 0 5 = sub address{2} 0 5
 ).
-
-(* ================================================== proof for gen leaf starts here =================================================================== *)
-
-inline {1} M(Syscall).__gen_leaf_wots_ M(Syscall)._gen_leaf_wots M(Syscall).__gen_leaf_wots.             
-
-seq 22 0 : (
-    #pre /\
-  sk_seed2{1} = sk_seed{1} /\
-  pub_seed2{1} = pub_seed{1} /\
-  ots_addr2{1} = ots_addr{1} /\
-  ltree_addr2{1} = ltree_addr{1}
-); first by auto.
-
-seq 1 1 : (
-        #{/~ots_addr2{1} = ots_addr{1}}pre /\ 
-        pk{1} = DecodeWotsPk pk{2} /\
-        ots_addr2{1}.[0] = address{2}.[0] /\
-        ots_addr2{1}.[1] = address{2}.[1] /\
-        ots_addr2{1}.[2] = address{2}.[2] /\
-        ots_addr2{1}.[3] = W32.zero 
-).
-         * exists * sk_seed2{1}, pub_seed2{1}, ots_addr2{1}, address{2}.
-           elim * => P3 P4 P5 P6.
-           call {1} (pkgen_correct P3 P4 P5 P6) => [/# |].
-           auto => /> &1 &2 H0 H1 H2 H3 H4 H5 H6 H7 H8 H9 H10 H11 H12 H13 H14 H15 H16 H17 H18 H19 H20 H21 H22 H23 H24 resL resR H25 H26*.
-           do split; [
-               have ->: P6.[0] = nth witness (sub P6 0 5) 0 by rewrite nth_sub | 
-               have ->: P6.[1] = nth witness (sub P6 0 5) 1 by rewrite nth_sub |     
-               have ->: P6.[2] = nth witness (sub P6 0 5) 2 by rewrite nth_sub |
-           ]; 1..3: by rewrite -H22 -H26 nth_sub /#.        
-           have ->: resL.`2.[3] = nth witness (sub resL.`2 0 5) 3 by rewrite nth_sub /#.
-           by rewrite H26 nth_sub.
-
-
-seq 0 2 : (
-          #{/~sub ots_addr{1} 0 5 = sub address{2} 0 5}pre /\ 
-          sub ltree_addr2{1} 0 5 = sub address{2} 0 5
-      ).
-         * auto => /> &1 &2 H0 H1 H2 H3 H4 H5 H6 H7 H8 H9 H10 H11 H12 H13 H14 H15 H16 H17 H18 H19 H20 H21 H22 H23 H24 H25 H26*.
-           rewrite /set_ltree_addr /set_type.
-           do split; (
-              apply (eq_from_nth witness); [by rewrite !size_sub | rewrite size_sub // => i?];
-              rewrite !nth_sub // !get_setE //=
-           ).
-               - do (rewrite ifF 1:/#).
-                 have ->: ltree_addr{1}.[i] = nth witness (sub ltree_addr{1} 0 3) i by rewrite nth_sub.
-                 by rewrite H11 nth_sub.
-               - do (rewrite ifF 1:/#).
-                 have ->: node_addr{1}.[i] = nth witness (sub node_addr{1} 0 3) i by rewrite nth_sub.
-                 by rewrite H12 nth_sub.
-               - case (i = 4) => [-> /# |?].
-                 case (i = 3) => [-> /# |?].
-                 do (rewrite ifF 1:/#).
-                 have ->: ltree_addr{1}.[i] = nth witness (sub ltree_addr{1} 0 3) i by rewrite nth_sub /#.
-                 by rewrite H11 nth_sub /#.
-
-
-seq 1 1 : (
-          #{/~ltree_addr2{1} = ltree_addr{1}}pre /\ 
-          to_list leaf1{1} = val node{2} /\
-          ltree_addr2{1}.[0] = address{2}.[0] /\
-          ltree_addr2{1}.[1] = address{2}.[1] /\
-          ltree_addr2{1}.[2] = address{2}.[2] /\
-          ltree_addr2{1}.[3] = W32.one
-      ).
-         * exists * pk{1}, ltree_addr2{1}, pub_seed2{1}.
-           elim * => P0 P1 P2.
-           call (ltree_correct P0 P2 P1) => [/# |].
-           auto => /> &1 &2 *; split; [apply enc_dec_wots_pk => /# | smt(addr_sub_5)].
-
-auto => /> &1 &2 H0 H1 H2 H3 H4 H5 H6 H7 H8 H9 H10 H11 H12 H13 H14 H15 H16 H17 H18 H19 H20 H21 H22 H23 H24 H25 H26 H27 H28 H29 H30 H31 *.
+    + exists * sk_seed{1}, pub_seed{1}, (of_int s{2})%W32, (of_int i{2})%W32, ots_addr{1}, ltree_addr{1}, address{2}.
+      elim * => P0 P1 P2 P3 P4 P5 P6.
+      call (gen_leaf_equiv P0 P1 P2 P3 P4 P5 P6) => [/# |].
+      skip => /> &1 &2 H0 H1 H2 H3 H4 H5 H6 H7 H8 H9 H10 H11 H12 H13 H14 H15 H16 H17 H18 H19 H20 H21 H22 H23 H24 H25 H26 H27 *.
       do split.
-         * apply (eq_from_nth witness); first by rewrite !size_sub.
-           rewrite size_sub // => i?. 
-           rewrite !nth_sub /#.
-         * by rewrite H28.
-         * apply (eq_from_nth witness); first by rewrite !size_sub.
-           rewrite size_sub // => i?. 
-           rewrite !nth_sub /#.
+        - apply (eq_from_nth witness); rewrite !size_sub // => j?; rewrite !nth_sub //; smt(sub_k).         
+        - smt(sub_k).
+        - smt(sub_k).
+        - rewrite -H23; smt(sub_k).
+        - smt(@NBytes).
+        - apply (eq_from_nth witness); rewrite !size_sub // => j?; rewrite !nth_sub //; smt(sub_k).         
 
-(* ================================================== proof for gen leaf ends here =================================================================== *)
- 
 seq 3 1 : (
         #{/~sub _stack{1} 0 (n * min (to_uint offset{2}) (size stack{2})) = sub_list (nbytes_flatten stack{2}) 0 (n * min (to_uint offset{2}) (size stack{2}))}pre /\
           sub _stack{1} 0 (n * min (to_uint offset{2} + 1) (size stack{2})) =
@@ -537,13 +482,15 @@ seq 3 1 : (
     + exists * buf{1}, stack{2}, _stack{1}, offset{1}.
       elim * => P0 P1 P2 P3. 
       sp.
-      call {1} (p_treehash_memcpy P0 P1 P2 P3) => [/# |].
-      skip => /> &1 &2 H0 H1 H2 H3 H4 H5 H6 H7 H8 H9 H10 H11 H12 H13 H14 H15 H16 H17 H18 H19 H20 H21 H22 *.
+      call {1} (p_treehash_memcpy_0 P0 P1 P2 P3) => [/# |].
+      skip => /> &1 &2 H0 H1 H2 H3 H4 H5 H6 H7 H8 H9 H10 H11 H12 H13 H14 H15 H16 H17 H18.
+      rewrite ultE => H19 H20 H21 H22 H23 *.
       do split. 
+        - smt(). 
+        - smt(@StdOrder.IntOrder).
+        - smt(). 
         - smt().
-        - smt(). 
-        - smt(). 
-        - move => H24 H25 H26 result H27 *.
+        - move => H H24 H25 H26 result H27 *.
           rewrite size_put; split => //. (* the first goal of split is solved by trivial *)
           apply (eq_from_nth witness); first by rewrite size_sub 1:/# size_sub_list /#.
           rewrite size_sub 1:/# => j?.
@@ -574,7 +521,7 @@ seq 1 1 : (
    sub heights{1} 0 (min (to_uint (offset{2} - W64.one)) (size heights{2})) = sub_list heights{2} 0 (min (to_uint (offset{2} - W64.one)) (size heights{2})) /\
    to_uint (offset{2} - W64.one) <= to_uint i{1}
 ).
-    + auto => /> &1 &2 H0 H1 H2 H3 H4 H5 H6 H7 H8 H9 H10 H11 H12 H13 H14 H15 H16 H17 H18 H19 H20 H21 H22 H23 *. 
+    + auto => /> &1 &2 H0 H1 H2 H3 H4 H5 H6 H7 H8 H9 H10 H11 H12 H13 H14 H15 H16 H17 H18 H19 H20 H21 H22 H23 H24*. 
       have E3: 0 <= to_uint i{1} <= 2 ^ 20 by smt(@RealExp).
       do split. 
       - rewrite to_uintD /= /#. (* This call to smt doesnt work without E1 in the context *)
@@ -588,14 +535,14 @@ seq 1 1 : (
             rewrite E1 n_val => j?.
             rewrite nth_sub //= /sub_list nth_mkseq //= nth_nbytes_flatten; first by smt(@W64 pow2_64).
             have ->: _stack{1}.[j] = nth witness (sub _stack{1} 0 (n * min (to_uint offset{2} + 1) (size stack{2}))) j by rewrite nth_sub; first by smt(@W64 pow2_64).
-            rewrite H23 /sub_list nth_mkseq; first by smt(@W64 pow2_64).
+            rewrite H24 /sub_list nth_mkseq; first by smt(@W64 pow2_64).
             rewrite /= nth_nbytes_flatten // /#.
           * have E1: min (to_uint (offset{2} + W64.one)) (size stack{2}) = size stack{2} by smt(@W64 pow2_64).
             rewrite E1 H9 d_val h_val n_val /= => j?. 
             rewrite nth_sub //.
             rewrite /sub_list nth_mkseq //= nth_nbytes_flatten 1:/#.
             have ->: _stack{1}.[j] = nth witness (sub _stack{1} 0 (n * min (to_uint offset{2} + 1) (size stack{2}))) j by rewrite nth_sub; first by smt(@W64 pow2_64).
-            rewrite H23 /sub_list nth_mkseq; first by smt(@W64 pow2_64).
+            rewrite H24 /sub_list nth_mkseq; first by smt(@W64 pow2_64).
             rewrite /= nth_nbytes_flatten // /#.
       - apply (eq_from_nth witness).  
           * rewrite size_sub; first by smt(@W64 pow2_64). 
@@ -605,12 +552,12 @@ seq 1 1 : (
         smt().
       - have ->: to_uint (offset{2} + W64.one - W64.one) = to_uint offset{2} by smt(@W64 pow2_64).
         apply H5.
-
+ 
 seq 1 1 : (
   #{/~sub heights{1} 0 (min (to_uint (offset{2} - W64.one)) (size heights{2})) = sub_list heights{2} 0 (min (to_uint (offset{2} - W64.one)) (size heights{2}))}pre /\
   sub heights{1} 0 (min (to_uint offset{2}) (size heights{2})) = sub_list heights{2} 0 (min (to_uint offset{2}) (size heights{2}))
 ).
-    + auto => /> &1 &2 H0 H1 H2 H3 H4 H5 H6 H7 H8 H9 H10 H11 H12 H13 H14 H15 H16 H17 H18 H19 H20 H21 H22 H23.
+    + auto => /> &1 &2 H0 H1 H2 H3 H4 H5 H6 H7 H8 H9 H10 H11 H12 H13 H14 H15 H16 H17 H18 H19 H20 H21 H22 H23 H24.
       rewrite size_put; split => //.
       apply (eq_from_nth witness).
          - rewrite size_sub; first by smt(@W64 pow2_64).
@@ -624,7 +571,7 @@ seq 1 1 : (
            case (j = to_uint (offset{2} - W64.one)) => [/# | ? //=].
            rewrite ifF 1:/#.
            have ->: heights{1}.[j] = nth witness (sub heights{1} 0 (min (to_uint (offset{2} - W64.one)) (size heights{2}))) j by rewrite nth_sub; smt(@W64 pow2_64).
-           rewrite H22 /sub_list nth_mkseq; first by smt(@W64 pow2_64).
+           rewrite H23 /sub_list nth_mkseq; first by smt(@W64 pow2_64).
            trivial.
          - have E1 : min (to_uint offset{2}) (size heights{2}) = size heights{2} by smt().
            rewrite E1 H9 h_val d_val /= => j?.
@@ -633,10 +580,8 @@ seq 1 1 : (
            rewrite get_set_if.
            rewrite ifF; first by smt(@W64 pow2_64).
            have ->: heights{1}.[j] = nth witness (sub heights{1} 0 (min (to_uint (offset{2} - W64.one)) (size heights{2}))) j by rewrite nth_sub; smt(@W64 pow2_64).
-           rewrite H22 /sub_list nth_mkseq; first by smt(@W64 pow2_64).
+           rewrite H23 /sub_list nth_mkseq; first by smt(@W64 pow2_64).
            trivial.
-
-conseq />.   
 
 seq 1 0 : (
     #pre /\ 
@@ -644,19 +589,19 @@ seq 1 0 : (
     (W64.of_int 2 \ule offset{2} /\ heights{1}.[to_uint (offset{1} - W64.of_int 2)] = heights{1}.[to_uint (offset{1} - W64.one)])
 ); first by  ecall {1} (p_treehash_condition_correct_eq heights{1} offset{1}); auto.
 
-seq 0 1 : (#{/~sub node_addr{1} 0 3 = sub address{2} 0 3}pre /\ sub node_addr{1} 0 5 = sub address{2} 0 5).
-  + auto => /> &1 &2 *.
-    rewrite /set_type.
-    do split; (
-      apply (eq_from_nth witness); [by rewrite !size_sub // | rewrite size_sub // => j?];
-      rewrite !nth_sub //= !get_setE //     
-    ).
-      - do rewrite ifF 1:/#; smt(sub_k).
-      - do rewrite ifF 1:/#; smt(sub_k).
-      - do 3! (rewrite ifF 1:/#).
-        case (j = 3) => [-> /# |?].
-        case (j = 4) => [-> /# |?].
-        smt(sub_k).
+seq 0 1 : (
+  #{/~sub ots_addr{1} 0 5 = sub address{2} 0 5}pre /\
+  sub ots_addr{1} 0 3 = sub address{2} 0 3 /\
+  sub node_addr{1} 0 5 = sub address{2} 0 5
+).
+    + auto => /> &1 &2 H0 H1 H2 H3 H4 H5 H6 H7 H8 H9 H10 H11 H12 H13 H14 H15 H16 H17 H18 H19 H20 H21 H22 H23 H24 H25.
+      rewrite /set_type.
+      do split; (apply (eq_from_nth witness); rewrite !size_sub // => j?; rewrite !nth_sub //= !get_setE //).
+        - rewrite !ifF 1..5:/#; smt(sub_k).
+        - rewrite !ifF 1..5:/#; smt(sub_k).
+        - rewrite !ifF 1..5:/#; smt(sub_k).
+        - rewrite ifF 1:/# ifF 1:/# ifF 1:/#.
+          smt(sub_k).
 
 while (
   t{2} = to_uint target_height{1} /\
@@ -666,8 +611,7 @@ while (
   0 <= s{2} <= h /\
 
   ={offset} /\
-  (0 < to_uint offset{2})/\
-    to_uint (offset{2} - W64.one) <= to_uint i{1} /\
+  (0 < to_uint offset{2}) /\ to_uint (offset{2} - W64.one) <= to_uint i{1} /\
   0 < i{2} <= 2 ^ t{2} /\
   to_uint i{1} = i{2} /\
   to_uint upper_bound{1} = 2 ^ t{2} /\
@@ -685,7 +629,7 @@ while (
   ots_addr{1}.[3] = W32.zero /\
   ltree_addr{1}.[3] = W32.one /\
   node_addr{1}.[3] = (of_int 2)%W32 /\
-  node_addr{1}.[4] = W32.zero /\
+  node_addr{1}.[4] = W32.zero /\ (* This is the padding value *)
 
   sub heights{1} 0 (min (to_uint offset{2}) (size heights{2})) = sub_list heights{2} 0 (min (to_uint offset{2}) (size heights{2})) /\
   sub _stack{1} 0 (n * (min (to_uint offset{2}) (size stack{2}))) = sub_list (nbytes_flatten stack{2}) 0 (n * (min (to_uint offset{2}) (size stack{2}))) /\
@@ -700,15 +644,14 @@ while (
 
 (* === the last subgoal of the second while starts here === *)
 
-auto => /> &1 &2 H0 H1 H2 H3 H4 H5 H6 H7 H8 H9 H10 H11 H12 H13 H14 H15 H16 H17 H18 H19 H20 H21 H22 H23 *.
+auto => /> &1 &2 H0 H1 H2 H3 H4 H5 H6 H7 H8 H9 H10 H11 H12 H13 H14 H15 H16 H17 H18 H19 H20 H21 H22 H23 H24 H25 H26.
 have E: forall (k : int), 0 <= k < (min (to_uint offset{2}) (size heights{2})) => heights{1}.[k] = nth witness heights{2} k.
         * move => k?.
           have ->: heights{1}.[k] = nth witness (sub heights{1} 0 (min (to_uint offset{2}) (size heights{2}))) k by rewrite nth_sub; smt(@W64 pow2_64).
-          by rewrite H22 /sub_list nth_mkseq.
-
+          by rewrite H23 /sub_list nth_mkseq.
 do split. 
     - smt(@W64 pow2_64).
-    - rewrite H23.
+    - rewrite H24.
       move => [#] Ha Hb.
       split; first by assumption.
       case (0 <= to_uint offset{2} < size heights{2}) => ?. (* offset - 2 e offset - 1 estao in bounds pq offset < size heights*)
@@ -732,7 +675,7 @@ do split.
                    apply Hc1.
               (* Por fim, esta tudo out of bounds *)
               by rewrite !nth_out.
-    - rewrite H23.
+    - rewrite H24.
       move => [#] Ha Hb.
       split; first by assumption.
       case (0 <= to_uint offset{2} < size heights{2}) => ?. (* offset - 2 e offset - 1 estao in bounds pq offset < size heights*)
@@ -755,13 +698,13 @@ do split.
                    rewrite (: size heights{2} = 11) 1:/# ; apply Hc1.
               (* Por fim, esta tudo out of bounds *)
               rewrite !get_out // /#.
-                
+
     - move => stackL condL heightsL nodeAdrL addressR heightsR offsetR stackR.
-      move => H25 H26 H27 H28 H29 H30 H31 H32 H33 HH35 H36 H37 H38 H39 *.
+      move => H27 H28 H29 H30 H31 H32 H33 H34 H35 H36 H37 H38 H39 H40 H41.
       have E3: 0 <= to_uint i{1} <= 2 ^ 20 by smt(@RealExp). (* Same as before *)
       do split.
         * rewrite to_uintD_small 1:/#.
-          have := H28.
+          have := H30.
           rewrite to_uintB; [by rewrite uleE /# => T |].
           smt(). (* Este smt so funciona depois de simplificarmos um bocado a hipotese H28 *)
         * smt().
@@ -833,13 +776,22 @@ seq 2 2 : (#pre /\ sub node_addr{1} 0 7 = sub address{2} 0 7).
             rewrite get_out; first by smt(@W64 pow2_64).
             reflexivity.
 
-
 seq 4 2 : (#pre /\ to_list buf2{1} = val node0{2} ++ val node1{2}).
     + sp.
       exists * _stack{1}, offset{1}, stack{2}.
       elim * => P0 P1 P2.
       call {1} (memcpy_treehash_node_2 P0 P1 P2) => [/# |].
-      skip => /> &1 &2 /#.
+      
+skip => /> &1 &2 H0 H1 H2 H3 H4 H5 H6 H7 H8 H9 H10 H11 H12 H13 H14 H15 H16 H17 H18 H19 H20 H21 H22 H23 H24 H25 *; do split => //=.
+        - smt().
+        - smt(@W64 pow2_64).
+        - rewrite h_val /=.
+        - move => ?.
+          move : H5.
+          have ->: to_uint (P1 - W64.one) = to_uint P1 - 1 by smt(@W64 pow2_64). (* Without this simplification, smt fails *)
+          move => H5.
+          smt(@StdOrder.IntOrder).
+        - smt().
 
 seq 1 1 : (#pre /\ to_list buf{1} = val new_node{2}).
           + inline M(Syscall).__thash_h_ M(Syscall)._thash_h.
@@ -861,23 +813,77 @@ seq 1 1 : (#pre /\ to_list buf{1} = val new_node{2}).
 ecall {1} (p_treehash_condition_correct_eq heights{1} offset{1}).
  
 conseq /> => [/# |].
- 
+
 seq 3 0 : (#pre /\ t64{1} = (offset{1} - (of_int 2)%W64) * (of_int 32)%W64); first by auto.
 
 seq 1 1 : #pre.
-    + exists * buf{1}, stack{2}, _stack{1}, offset{2}.
+    + exists * buf{1}, stack{2}, _stack{1}, (offset{1} - (of_int 2)%W64).
       elim * => P0 P1 P2 P3.  
-      call {1} (p_treehash_memcpy_2 P0 P1 P2 P3) => [/# |].
-      auto => /> &1 &2 H0 H1 H2 H3 H4 H5 H6 H7 H8 H9 H10 H11 H12 H13 H14 H15 H16 H17 H18 H19 H20 H21 H22 H23 H24 H25 H26 *.
+      call {1} (p_treehash_memcpy P0 P1 P2 P3) => [/# |].
+      auto => /> &1 &2 H0 H1 H2 H3 H4 H5 H6 H7 H8 H9 H10 H11 H12 H13 H14 H15 H16 H17 H18 H19 H20 H21 H22.
+      rewrite uleE of_uintK /= => H23 H24 H25 H26 H27 *.
       rewrite !size_put.
-      do split.
-        - smt(@W64 pow2_64).
+      do split. 
+        - smt(@W64 pow2_64). 
+        - move : H5.
+          have ->: to_uint (offset{2} - W64.one) = to_uint offset{2} - 1 by smt(@W64 pow2_64). (* Without this simplification, smt fails *)
+          move => H5.
+          have ->: to_uint (offset{2} - (of_int 2)%W64) = to_uint offset{2} - 2 by smt(@W64 pow2_64). 
+          smt(@StdOrder.IntOrder).
         - smt(). 
-        - move => H27 H28 result ->.
-          split => //.
-          do congr.
-          smt(@NBytes).
- 
+        - have ->: to_uint (offset{2} - (of_int 2)%W64) = to_uint offset{2} - 2 by smt(@W64 pow2_64).
+          apply (eq_from_nth witness).
+             * rewrite size_sub 1:/# size_sub_list /#.
+          rewrite size_sub 1:/# /XMSS_N /= => i?. 
+          rewrite -n_val.
+          by rewrite H19 !nth_mkseq 1,2:/#. 
+        - rewrite /XMSS_N n_val => H29 H28 Ha Hb result Hr.  
+          split => [/# |].
+          have ->: new_node{2} = NBytes.insubd (to_list P0) by smt(@NBytes).
+          have E: to_uint (offset{2} - (of_int 2)%W64) = to_uint offset{2} - 2 by smt(@W64 pow2_64). 
+          rewrite E.
+          apply (eq_from_nth witness); first by rewrite size_sub 1:/# size_sub_list 1:/#.
+          rewrite size_sub 1:/# => j?.          
+          rewrite !nth_sub //= nth_mkseq  //= nth_nbytes_flatten; first by rewrite size_put /#.
+
+          case (0 <= to_uint offset{2} - 2 < size P1) => [H_o_m_2_in | H_o_m_2_out]; last first.
+             * rewrite put_out 1:/#. 
+               have ->: result.[j] =
+                        nth witness 
+                        (sub result 0 (32 * min (to_uint (offset{2} - (of_int 2)%W64) + 1) (size P1)))   
+                        j by rewrite E /= nth_sub // /#.
+               rewrite E nth_mkseq 1:/# /=. 
+               have ->: result.[j] = 
+                        nth witness (sub result 0
+                                        (32 * min (to_uint (offset{2} - (of_int 2)%W64) + 2) (size P1))
+                        ) j by rewrite nth_sub //; smt(@W64 pow2_64).
+               rewrite Hr nth_sub_list 1:/#.
+               rewrite  nth_nbytes_flatten; first by rewrite size_put /#.
+               rewrite put_out 2:/#; smt(@W64 pow2_64).
+
+             * rewrite nth_put //. 
+               case (to_uint offset{2} - 2 = j %/ n) => [H_a | H_b].
+                   + rewrite H27 insubdK; first by rewrite /P valP.
+                     have ->: result.[j] =
+                              nth witness 
+                              (sub result 0 (32 * min (to_uint (offset{2} - (of_int 2)%W64) + 2) (size P1)))   
+                              j by rewrite E /= nth_sub // /#.
+                    
+                     rewrite Hr E nth_mkseq /= 1:/# nth_nbytes_flatten; first by rewrite size_put /#.
+                     by rewrite nth_put 1:/# ifT 1:/# H27 insubdK // /P valP.
+                   + case (0 <= j && j < 32 * min (to_uint offset{2} - 1) (size P1)) => [Hba | Hbb].
+                      * have ->: result.[j] = nth witness
+                                 (sub result 0 (32 * min (to_uint (offset{2} - (of_int 2)%W64) + 2) (size P1))) 
+                                 j by rewrite E nth_sub 1:/#.  
+                        rewrite Hr E nth_mkseq 1:/# /= nth_nbytes_flatten; first by rewrite size_put /#.
+                        rewrite nth_put 1:/# ifF 1:/#; reflexivity.
+                      * have ->: result.[j] = nth witness
+                                 (sub result 0 (32 * min (to_uint (offset{2} - (of_int 2)%W64) + 2) (size P1))) 
+                                 j by rewrite E nth_sub 1:/#.  
+                        rewrite Hr E nth_mkseq 1:/# /= nth_nbytes_flatten; first by rewrite size_put /#.
+                        rewrite nth_put 1:/# ifF 1:/#; reflexivity.
+
+
 auto => /> &1 &2 H0 H1 H2 H3 H4 H5 H6 H7 H8 H9 H10 H11 H12 H13 H14 H15 H16 H17 H18 H19 H20 H21 H22 H23 H24 H25 H26 H27 cond ->.
 rewrite !size_put /treehash_cond.
 do split => //.
